add aux thms

Barrel/Builtins/Function.lean
@@ -1,43 +1,240 @@
 import Barrel.Builtins.Relation
+import Batteries.Tactic.GeneralizeProofs
 
 namespace B.Builtins
   abbrev pfun {α β : Type _} (A : Set α) (B : Set β) : Set (SetRel α β) :=
-    { f : Set (α × β) | f ∈ rels A B ∧ ∀ ⦃x y z⦄, (x, y) ∈ f → (x, z) ∈ f → y = z }
+    { f : Set (α × β) | f ∈ A ⟷ B ∧ ∀ ⦃x y z⦄, (x, y) ∈ f → (x, z) ∈ f → y = z }
   scoped infixl:125 " ⇸ " => pfun
 
   abbrev tfun {α β : Type _} (A : Set α) (B : Set β) : Set (SetRel α β) :=
-    { f : Set (α × β) | f ∈ pfun A B ∧ ∀ x ∈ A, ∃ y ∈ B, (x, y) ∈ f }
+    { f : Set (α × β) | f ∈ A ⇸ B ∧ ∀ x ∈ A, ∃ y ∈ B, (x, y) ∈ f }
   scoped infixl:125 " ⟶ " => tfun
 
   abbrev injPFun {α β : Type _} (A : Set α) (B : Set β) : Set (SetRel α β) :=
-    { f : Set (α × β) | f ∈ pfun A B ∧ ∀ ⦃x₁ x₂ y⦄, (x₁, y) ∈ f → (x₂, y) ∈ f → x₁ = x₂ }
+    { f : Set (α × β) | f ∈ A ⇸ B ∧ ∀ ⦃x₁ x₂ y⦄, (x₁, y) ∈ f → (x₂, y) ∈ f → x₁ = x₂ }
   scoped infixl:125 " ⤔ " => injPFun
 
   abbrev injTFun {α β : Type _} (A : Set α) (B : Set β) : Set (SetRel α β) :=
-    injPFun A B ∩ tfun A B
+    A ⤔ B ∩ A ⟶ B
   scoped infixl:125 " ↣ " => injTFun
 
   abbrev surjPFun {α β : Type _} (A : Set α) (B : Set β) : Set (SetRel α β) :=
-    { f : Set (α × β) | f ∈ pfun A B ∧ ∀ y ∈ B, ∃ x ∈ A, (x, y) ∈ f }
+    { f : Set (α × β) | f ∈ A ⇸ B ∧ ∀ y ∈ B, ∃ x ∈ A, (x, y) ∈ f }
   scoped infixl:125 " ⤀ " => surjPFun
 
   abbrev surjTFun {α β : Type _} (A : Set α) (B : Set β) : Set (SetRel α β) :=
-    surjPFun A B ∩ tfun A B
+    A ⤀ B ∩ A ⟶ B
   scoped infixl:125 " ↠ " => surjTFun
 
   abbrev bijPFun {α β : Type _} (A : Set α) (B : Set β) : Set (SetRel α β) :=
-    injPFun A B ∩ surjPFun A B
+    A ⤔ B ∩ A ⤀ B
   scoped infixl:125 " ⤗ " => bijPFun
 
   abbrev bijTFun {α β : Type _} (A : Set α) (B : Set β) : Set (SetRel α β) :=
-    injTFun A B ∩ surjTFun A B
+    A ↣ B ∩ A ↠ B
   scoped infixl:125 " ⤖ " => bijTFun
 
   structure app.WF {α : Type _} {β : Type _} (f : SetRel α β) (x : α) : Prop where
-    isPartialFunction : f ∈ pfun (dom f) (ran f)
+    isPartialFunction : f ∈ dom f ⟶ ran f
     isInDomain : x ∈ dom f
 
-  noncomputable abbrev app {α β : Type _} (f : SetRel α β) (x : α) (wf : app.WF f x): β :=
+  noncomputable abbrev app {α β : Type _} (f : SetRel α β) (x : α) (wf : app.WF f x) : β :=
     Classical.choose wf.isInDomain
   scoped notation:290 F:290 "(" x:min ")'" wf:300 => app F x wf
+
+  section Lemmas
+
+    @[grind .]
+    theorem pfun_of_singleton {α β : Type _} {a : α} {b : β} :
+        {(a, b)} ∈ {a} ⇸ {b} := by
+      and_intros
+      · rintro ⟨x, y⟩ hxy
+        rw [Set.mem_singleton_iff] at hxy
+        obtain ⟨rfl, rfl⟩ := hxy
+        trivial
+      · intro x y z hxy hxz
+        rw [Set.mem_singleton_iff] at hxy hxz
+        obtain ⟨rfl, rfl⟩ := hxy
+        obtain ⟨rfl, rfl⟩ := hxz
+        rfl
+
+    @[grind .]
+    theorem tfun_of_singleton {α β : Type _} {a : α} {b : β} :
+        {(a, b)} ∈ {a} ⟶ {b} := by
+      constructor
+      · exact pfun_of_singleton
+      · rintro _ rfl
+        exists b
+
+    @[grind .]
+    theorem pfun_singleton {α β : Type _} {a : α} {b : β} {A : Set α} {B : Set β}
+      (ha : a ∈ A) (hb : b ∈ B) :
+        {(a, b)} ∈ A ⇸ B := by
+      and_intros
+      · rintro ⟨x, y⟩ hxy
+        rw [Set.mem_singleton_iff] at hxy
+        obtain ⟨rfl, rfl⟩ := hxy
+        trivial
+      · intro x y z hxy hxz
+        rw [Set.mem_singleton_iff] at hxy hxz
+        obtain ⟨rfl, rfl⟩ := hxy
+        obtain ⟨rfl, rfl⟩ := hxz
+        rfl
+
+    theorem app.WF_of_mem_pfun {α β : Type _} {f : SetRel α β} {A : Set α} {B : Set β} {x : α} (hf : f ∈ A ⇸ B) (hA : A ⊆ dom f) (hx : x ∈ A) :
+      app.WF f x where
+      isPartialFunction := by
+        obtain ⟨f_rel, f_is_func⟩ := hf
+        and_intros
+        · rintro ⟨x, y⟩ hxy
+          and_intros
+          · exists y
+          · exists x
+        · exact fun _ _ _ ↦ (f_is_func · ·)
+        · intro x hx
+          obtain ⟨y, hxy⟩ := hx
+          refine ⟨y, ?_, hxy⟩
+          rw [Set.mem_setOf]
+          exists x
+      isInDomain := hA hx
+
+    theorem app.WF_of_mem_dom_pfun {α β : Type _} {f : SetRel α β} {A : Set α} {B : Set β} {x : α} (hf : f ∈ A ⇸ B) (hx : x ∈ dom f) :
+      app.WF f x where
+      isPartialFunction := by
+        obtain ⟨f_rel, f_is_func⟩ := hf
+        and_intros
+        · rintro ⟨x, y⟩ hxy
+          and_intros
+          · exists y
+          · exists x
+        · exact fun _ _ _ ↦ (f_is_func · ·)
+        · intro x hx
+          obtain ⟨y, hxy⟩ := hx
+          refine ⟨y, ?_, hxy⟩
+          rw [Set.mem_setOf]
+          exists x
+      isInDomain := hx
+
+    theorem app.WF_of_mem_tfun {α β : Type _} {f : SetRel α β} {A : Set α} {B : Set β} {x : α}
+      (hf : f ∈ A ⟶ B) (hx : x ∈ A) :
+        app.WF f x := by
+      apply app.WF_of_mem_pfun hf.1 (fun y hy ↦ ?_) hx
+      · obtain ⟨z, -, hfxy⟩ := hf.2 y hy
+        exact ⟨z, hfxy⟩
+
+    @[grind →, simp]
+    theorem app.of_pair_eq {α β : Type _} {f : SetRel α β} {x : α} {y : β}
+      (wf : WF f x) (hxy : (x, y) ∈ f) :
+        app f x wf = y :=
+          wf.isPartialFunction.1.2 hxy (Classical.choose_spec wf.isInDomain) |>.symm
+
+    @[grind →]
+    theorem app.pair_app_mem {α β : Type _} {f : SetRel α β} {x : α} {wf : WF f x} :
+      (x, f(x)'wf) ∈ f := Classical.choose_spec wf.isInDomain
+
+    @[grind =, simp]
+    theorem app.of_pair_iff {α β : Type _} {f : SetRel α β} {x : α} {y : β}
+      (wf : WF f x) :
+        (x, y) ∈ f ↔ app f x wf = y where
+      mp hxy := app.of_pair_eq wf hxy
+      mpr h_eq := by
+        rw [←h_eq]
+        exact pair_app_mem
+
+    @[simp]
+    theorem tfun_dom_eq {α β : Type _} {A : Set α} {B : Set β} {f : SetRel α β} (hf : f ∈ A ⟶ B) :
+      dom f = A := by
+        ext x
+        constructor <;> intro h
+        · obtain ⟨_, hy⟩ := h
+          exact hf.1.1 _ hy |>.1
+        · obtain ⟨_, -, hy⟩ := hf.2 x h
+          exact mem_dom_of_pair_mem hy
+
+    @[simp]
+    theorem overload_dom_eq {α β : Type _} {R₁ R₂ : SetRel α β} :
+        dom (R₁ <+ R₂) = dom R₁ ∪ dom R₂ := by
+      ext x
+      constructor <;> intro h
+      · rw [Set.mem_setOf_eq] at h
+        obtain ⟨y, hy⟩ := h
+        rw [Set.mem_setOf_eq] at hy
+        obtain ⟨mem_R₁, -⟩ | ⟨mem_R₂⟩ := hy
+        · left
+          exists y
+        · right
+          exists y
+      · by_cases hx : x ∈ dom R₂
+        · obtain ⟨y, hy⟩ := hx
+          exists y
+          right
+          exact hy
+        · obtain h | h := h
+          · obtain ⟨y, hy⟩ := h
+            rw [Set.mem_setOf_eq]
+            exists y
+            simp only [overload, Set.mem_setOf, not_exists]
+            left
+            and_intros
+            · exact hy
+            · simpa [Set.mem_setOf_eq, not_exists] using hx
+          · nomatch hx h
+
+    theorem pfun_of_overload {α β : Type _} {A C : Set α} {B D : Set β} {f₁ f₂ : SetRel α β}
+      (hf₁ : f₁ ∈ A ⇸ B) (hf₂ : f₂ ∈ C ⇸ D) :
+        f₁ <+ f₂ ∈ (A ∪ C) ⇸ (B ∪ D) := by
+      and_intros
+      · rintro ⟨x, y⟩ hxy
+        simp only [overload, Set.mem_setOf, not_exists] at hxy
+        obtain ⟨mem_f₁, notmem_f₂⟩ | mem_f₂ := hxy
+        · and_intros
+          · left
+            exact hf₁.1 _ mem_f₁ |>.1
+          · left
+            exact hf₁.1 _ mem_f₁ |>.2
+        · and_intros
+          · right
+            exact hf₂.1 _ mem_f₂ |>.1
+          · right
+            exact hf₂.1 _ mem_f₂ |>.2
+      · intro x y z hxy hxz
+        simp only [overload, Set.mem_setOf, not_exists] at hxy hxz
+        obtain ⟨mem_f₁, notmem_f₂⟩ | mem_f₂ := hxy
+        · obtain ⟨mem_f₁', notmem_f₂'⟩ | mem_f₂' := hxz
+          · exact hf₁.2 mem_f₁ mem_f₁'
+          · nomatch notmem_f₂ _ mem_f₂'
+        · obtain ⟨mem_f₁', notmem_f₂'⟩ | mem_f₂' := hxz
+          · nomatch notmem_f₂' _ mem_f₂
+          · exact hf₂.2 mem_f₂ mem_f₂'
+
+    theorem app.WF_of_overload {α β : Type _} {A C : Set α} {B D : Set β} {f₁ f₂ : SetRel α β}
+      {x : α} (hf₁ : f₁ ∈ A ⇸ B) (hf₂ : f₂ ∈ C ⇸ D) (hx : x ∈ dom f₁ ∨ x ∈ dom f₂) :
+        app.WF (f₁ <+ f₂) x := by
+      obtain hx | hx := hx <;> {
+        apply app.WF_of_mem_dom_pfun
+        · apply pfun_of_overload hf₁ hf₂
+        · rw [overload_dom_eq]
+          grind
+      }
+
+    theorem tfun_of_overload {α β : Type _} {A C : Set α} {B D : Set β} {f g : SetRel α β}
+      (hf : f ∈ A ⟶ B) (hg : g ∈ C ⟶ D) :
+        f <+ g ∈ (A ∪ C) ⟶ (B ∪ D) := by
+      refine ⟨pfun_of_overload hf.1 hg.1, ?_⟩
+      rintro x hx
+      by_cases x_dom : x ∈ dom g
+      · obtain ⟨y, hy⟩ := x_dom
+        exists y, ?_ <;> right
+        · exact hg.1.1 _ hy |>.2
+        · exact hy
+      · rw [tfun_dom_eq hg] at x_dom
+        replace hx := Or.resolve_right hx x_dom
+        rw [←tfun_dom_eq hf] at hx
+        obtain ⟨y, hy⟩ := hx
+        exists y, ?_ <;> left
+        · exact hf.1.1 _ hy |>.2
+        · rw [tfun_dom_eq hg]
+          exact ⟨hy, x_dom⟩
+
+  end Lemmas
 end B.Builtins
