Barrel/Builtins/Arithmetic.lean
@@ -26,86 +26,184 @@ namespace B.Builtins
 
   section Lemmas
 
-  @[grind=, simp]
-  theorem interval.of_singleton_eq (a : ℤ) : (a .. a) = {a} :=
-    Set.Icc_self a
+    @[grind =, simp]
+    theorem NAT.eq_interval : NAT = (0 .. MAXINT) := rfl
 
-  theorem interval.finite (lo hi : ℤ) : (lo .. hi).Finite := Set.finite_Icc lo hi
+    @[grind =, simp]
+    theorem NAT₁.eq_interval : NAT₁ = (1 .. MAXINT) := rfl
 
-  theorem interval.nonempty {lo hi : ℤ} (h : lo ≤ hi) : (lo .. hi).Nonempty :=
-    Set.nonempty_Icc.mpr h
+    @[grind =, simp]
+    theorem INT.eq_interval : INT = (MININT .. MAXINT) := rfl
 
-  theorem interval.FIN₁_mem {lo hi : ℤ} (h : lo ≤ hi) : lo .. hi ∈ FIN₁ INTEGER := by
-    and_intros
-    · exact fun _ _ => trivial
-    · exact finite lo hi
-    · exact nonempty h
+    @[grind=, simp]
+    theorem interval.of_singleton_eq (a : ℤ) : (a .. a) = {a} :=
+      Set.Icc_self a
 
-  @[grind., simp]
-  theorem min.WF_NATURAL : min.WF NATURAL := by
-    exists 0
-    and_intros
-    · rw [Builtins.NATURAL, Set.mem_setOf]
-    · intro y hy
-      rwa [Set.mem_setOf] at hy
+    @[grind .]
+    theorem interval.finite (lo hi : ℤ) : (lo .. hi).Finite := Set.finite_Icc lo hi
 
-  theorem min.WF_of_finite {α : Type _} [LinearOrder α] {S A : Set α} (h : S ∈ FIN₁ A) :
-      min.WF S := by
-    let fin := Set.Finite.to_subtype h.1.2
-    let nemp := Set.Nonempty.to_subtype h.2
-    obtain ⟨x, h⟩ := Finite.exists_min (@_root_.id ↑S)
-    exact ⟨x, Subtype.coe_prop x, fun y hy ↦ h ⟨y, hy⟩⟩
+    @[grind .]
+    theorem interval.nonempty {lo hi : ℤ} (h : lo ≤ hi) : (lo .. hi).Nonempty :=
+      Set.nonempty_Icc.mpr h
 
-  theorem max.WF_of_finite {α : Type _} [LinearOrder α] {S A : Set α} (h : S ∈ FIN₁ A) :
-      max.WF S := by
-    let fin := Set.Finite.to_subtype h.1.2
-    let nemp := Set.Nonempty.to_subtype h.2
-    obtain ⟨x, h⟩ := Finite.exists_max (@_root_.id ↑S)
-    exact ⟨x, Subtype.coe_prop x, fun y hy ↦ h ⟨y, hy⟩⟩
+    theorem interval.FIN_mem {lo hi : ℤ} : lo .. hi ∈ FIN INTEGER := by
+      and_intros
+      · exact fun _ _ => trivial
+      · exact finite lo hi
 
-  theorem max.WF_interval {lo hi : ℤ} (h : lo ≤ hi) : max.WF (lo..hi) := by
-    exists hi
-    and_intros <;> grind
+    theorem interval.FIN₁_mem {lo hi : ℤ} (h : lo ≤ hi) : lo .. hi ∈ FIN₁ INTEGER :=
+      ⟨FIN_mem, interval.nonempty h⟩
 
-  theorem min.WF_interval {lo hi : ℤ} (h : lo ≤ hi) : min.WF (lo..hi) := by
-    exists lo
-    and_intros <;> grind
 
-  @[grind ., simp]
-  theorem interval.min_eq {lo hi : Int} (h : lo ≤ hi) :
-      min (lo .. hi) (min.WF_interval h) = lo := by
-    unfold min
-    generalize_proofs hm
-    obtain ⟨m_def, m_is_min⟩ := Classical.choose_spec hm
-    exact le_antisymm (m_is_min _ (Set.left_mem_Icc.mpr h)) m_def.1
+    @[grind .]
+    theorem NAT.Finite : NAT.Finite := by
+      rw [eq_interval]
+      apply interval.finite
 
-  @[grind ., simp]
-  theorem interval.max_eq {lo hi : Int} (h : lo ≤ hi) :
-      max (lo .. hi) (max.WF_interval h) = hi := by
-    unfold max
-    generalize_proofs hm
-    obtain ⟨m_def, m_is_max⟩ := Classical.choose_spec hm
-    exact le_antisymm m_def.2 (m_is_max _ (Set.right_mem_Icc.mpr h))
+    @[grind .]
+    theorem NAT.mem_FIN : NAT ∈ FIN INTEGER := interval.FIN_mem
 
-  theorem min.WF_singleton {α : Type _} [LinearOrder α] {a : α} : min.WF {a} :=
-    min.WF_of_finite <| FIN₁.singleton_mem (Set.mem_singleton a)
+    @[grind .]
+    theorem NAT.mem_FIN₁ : NAT ∈ FIN₁ INTEGER := interval.FIN₁_mem (Int.zero_le_ofNat _)
 
-  theorem max.WF_singleton {α : Type _} [LinearOrder α] {a : α} : max.WF {a} :=
-    max.WF_of_finite <| FIN₁.singleton_mem (Set.mem_singleton a)
+    @[grind =, simp]
+    theorem NAT.pow_eq_fin : 𝒫 NAT = FIN NAT := by
+      ext S
+      rw [eq_interval, Set.mem_powerset_iff]
+      constructor <;> intro hS
+      · exact FIN.of_sub ⟨subset_refl _, interval.finite _ _⟩ hS
+      · exact hS.1
 
-  @[simp]
-  theorem min.of_singleton {α : Type _} [LinearOrder α] {a : α} :
-      min {a} (min.WF_singleton) = a := by
-    unfold min
-    generalize_proofs ha
-    exact (Classical.choose_spec ha).1
+    @[grind =, simp]
+    theorem NAT₁.pow_eq_fin : 𝒫 NAT₁ = FIN NAT₁ := by
+      ext S
+      rw [eq_interval, Set.mem_powerset_iff]
+      constructor <;> intro hS
+      · exact FIN.of_sub ⟨subset_refl _, interval.finite _ _⟩ hS
+      · exact hS.1
 
-  @[simp]
-  theorem max.of_singleton {α : Type _} [LinearOrder α] {a : α} :
-      max {a} (max.WF_singleton) = a := by
-    unfold max
-    generalize_proofs ha
-    exact (Classical.choose_spec ha).1
+    @[grind =, simp]
+    theorem INT.pow_eq_fin : 𝒫 INT = FIN INT := by
+      ext S
+      rw [eq_interval, Set.mem_powerset_iff]
+      constructor <;> intro hS
+      · exact FIN.of_sub ⟨subset_refl _, interval.finite _ _⟩ hS
+      · exact hS.1
+
+    @[grind =, simp]
+    theorem NAT.pow₁_eq_fin₁ : 𝒫₁ NAT = FIN₁ NAT := by
+      ext S
+      rw [eq_interval, Set.mem_setOf_eq, Set.mem_powerset_iff]
+      constructor <;> intro hS
+      · apply FIN₁.of_sub
+        · exact FIN₁.of_finite_nonempty_self
+            (interval.finite _ _)
+            (interval.nonempty (Int.zero_le_ofNat _))
+        · exact hS.1
+        · exact hS.2
+      · exact ⟨hS.1.1, hS.2⟩
+
+    @[grind =, simp]
+    theorem NAT₁.pow₁_eq_fin₁ : 𝒫₁ NAT₁ = FIN₁ NAT₁ := by
+      ext S
+      rw [eq_interval, Set.mem_setOf_eq, Set.mem_powerset_iff]
+      constructor <;> intro hS
+      · apply FIN₁.of_sub
+        · exact FIN₁.of_finite_nonempty_self
+            (interval.finite _ _)
+            (interval.nonempty (Int.zero_le_ofNat _))
+        · exact hS.1
+        · exact hS.2
+      · exact ⟨hS.1.1, hS.2⟩
+
+    @[grind =, simp]
+    theorem INT.pow₁_eq_fin₁ : 𝒫₁ INT = FIN₁ INT := by
+      ext S
+      rw [eq_interval, Set.mem_setOf_eq, Set.mem_powerset_iff]
+      constructor <;> intro hS
+      · apply FIN₁.of_sub
+        · exact FIN₁.of_finite_nonempty_self
+            (interval.finite _ _)
+            (interval.nonempty (Int.zero_le_ofNat _))
+        · exact hS.1
+        · exact hS.2
+      · exact ⟨hS.1.1, hS.2⟩
+
+    @[grind .]
+    theorem NAT₁.Finite : NAT₁.Finite := by
+      rw [eq_interval]
+      apply interval.finite
+
+    @[grind .]
+    theorem INT.Finite : INT.Finite := by
+      rw [eq_interval]
+      apply interval.finite
+
+    @[grind., simp]
+    theorem min.WF_NATURAL : min.WF NATURAL := by
+      exists 0
+      and_intros
+      · rw [Builtins.NATURAL, Set.mem_setOf]
+      · intro y hy
+        rwa [Set.mem_setOf] at hy
+
+    theorem min.WF_of_finite {α : Type _} [LinearOrder α] {S A : Set α} (h : S ∈ FIN₁ A) :
+        min.WF S := by
+      let fin := Set.Finite.to_subtype h.1.2
+      let nemp := Set.Nonempty.to_subtype h.2
+      obtain ⟨x, h⟩ := Finite.exists_min (@_root_.id ↑S)
+      exact ⟨x, Subtype.coe_prop x, fun y hy ↦ h ⟨y, hy⟩⟩
+
+    theorem max.WF_of_finite {α : Type _} [LinearOrder α] {S A : Set α} (h : S ∈ FIN₁ A) :
+        max.WF S := by
+      let fin := Set.Finite.to_subtype h.1.2
+      let nemp := Set.Nonempty.to_subtype h.2
+      obtain ⟨x, h⟩ := Finite.exists_max (@_root_.id ↑S)
+      exact ⟨x, Subtype.coe_prop x, fun y hy ↦ h ⟨y, hy⟩⟩
+
+    theorem max.WF_interval {lo hi : ℤ} (h : lo ≤ hi) : max.WF (lo..hi) := by
+      exists hi
+      and_intros <;> grind
+
+    theorem min.WF_interval {lo hi : ℤ} (h : lo ≤ hi) : min.WF (lo..hi) := by
+      exists lo
+      and_intros <;> grind
+
+    @[grind ., simp]
+    theorem interval.min_eq {lo hi : Int} (h : lo ≤ hi) :
+        min (lo .. hi) (min.WF_interval h) = lo := by
+      unfold min
+      generalize_proofs hm
+      obtain ⟨m_def, m_is_min⟩ := Classical.choose_spec hm
+      exact le_antisymm (m_is_min _ (Set.left_mem_Icc.mpr h)) m_def.1
+
+    @[grind ., simp]
+    theorem interval.max_eq {lo hi : Int} (h : lo ≤ hi) :
+        max (lo .. hi) (max.WF_interval h) = hi := by
+      unfold max
+      generalize_proofs hm
+      obtain ⟨m_def, m_is_max⟩ := Classical.choose_spec hm
+      exact le_antisymm m_def.2 (m_is_max _ (Set.right_mem_Icc.mpr h))
+
+    theorem min.WF_singleton {α : Type _} [LinearOrder α] {a : α} : min.WF {a} :=
+      min.WF_of_finite <| FIN₁.singleton_mem (Set.mem_singleton a)
+
+    theorem max.WF_singleton {α : Type _} [LinearOrder α] {a : α} : max.WF {a} :=
+      max.WF_of_finite <| FIN₁.singleton_mem (Set.mem_singleton a)
+
+    @[simp]
+    theorem min.of_singleton {α : Type _} [LinearOrder α] {a : α} :
+        min {a} (min.WF_singleton) = a := by
+      unfold min
+      generalize_proofs ha
+      exact (Classical.choose_spec ha).1
+
+    @[simp]
+    theorem max.of_singleton {α : Type _} [LinearOrder α] {a : α} :
+        max {a} (max.WF_singleton) = a := by
+      unfold max
+      generalize_proofs ha
+      exact (Classical.choose_spec ha).1
 
   end Lemmas
 end B.Builtins
