Barrel/Builtins/Power.lean
@@ -1,3 +1,4 @@
+import Barrel.Builtins.Init
 import Mathlib.Data.Set.Basic
 import Mathlib.Data.Finite.Defs
 import Mathlib.Data.Set.Finite.Basic
@@ -11,9 +12,44 @@ namespace B.Builtins
 
   section Lemmas
 
+    @[grind .]
+    theorem FIN.of_finite_self {α : Type _} {A : Set α} (hA : A.Finite) : A ∈ FIN A :=
+      ⟨subset_refl _, hA⟩
+
+    @[grind .]
+    theorem FIN₁.of_finite_nonempty_self {α : Type _} {A : Set α} (h : A.Finite) (h' : A.Nonempty) :
+      A ∈ FIN₁ A := ⟨⟨subset_refl _, h⟩, h'⟩
+
     theorem FIN₁.singleton_mem {α : Type _} {a : α} {A : Set α} (ha : a ∈ A) :
         {a} ∈ FIN₁ A := by
       simpa
 
+    theorem FIN.of_sub {α : Type _} {A B : Set α} {S : Set α} (h : S ∈ FIN A) (hsub : B ⊆ S) :
+        B ∈ FIN A := by
+      rw [Set.mem_setOf] at h ⊢
+      obtain ⟨hS, Sfin⟩ := h
+      and_intros
+      · trans S
+        · exact hsub
+        · exact hS
+      · exact Set.Finite.subset Sfin hsub
+
+    theorem FIN₁.of_sub {α : Type _} {A B : Set α} {S : Set α} (h : S ∈ FIN₁ A) (hsub : B ⊆ S) (hB : B.Nonempty) :
+        B ∈ FIN₁ A := by
+      rw [Set.mem_setOf] at h ⊢
+      obtain ⟨⟨hS, Sfin⟩, Snemp⟩ := h
+      exact ⟨⟨fun _ => (hS <| hsub ·), Set.Finite.subset Sfin hsub⟩, hB⟩
+
+    theorem FIN.of_inter {α : Type _} {A B : Set α} {S : Set α} (h : A ∈ FIN S ∨ B ∈ FIN S) :
+        A ∩ B ∈ FIN S := by
+      obtain h | h := h
+        <;> [ skip ; rw [Set.inter_comm] ]
+        <;> exact FIN.of_sub h Set.inter_subset_left
+
+    theorem FIN₁.of_inter {α : Type _} {A B : Set α} {S : Set α} (h : A ∈ FIN₁ S ∨ B ∈ FIN₁ S) :
+        A ∩ B ∈ FIN S := by
+      obtain h | h := h
+        <;> [ skip ; rw [Set.inter_comm] ]
+        <;> exact FIN.of_sub (Set.mem_of_mem_inter_left h) Set.inter_subset_left
   end Lemmas
 end B.Builtins
